Hoare.v
@@ -1,0 +1,108 @@
+(** Crash Hoare Logic specifications *)
+
+(* TODO: document how specifications are structured *)
+
+Require Import Automation.
+Require Import Prog.
+Require Import ProgTheorems.
+
+Set Implicit Arguments.
+
+Record Quadruple T :=
+  Spec {
+      pre: Prop;
+      post: T -> PState -> Prop;
+      crash: PState -> Prop;
+    }.
+
+(** A specification quantifies over ghost state of type A, and gives pre/post
+conditions and crash invariant specialized to a particular initial state. (This
+is why [pre] above is just a [Prop].) *)
+Definition Specification A T := A -> PState -> Quadruple T.
+
+Definition prog_spec T A (spec: Specification A T) (p: prog3 T) :=
+  forall a pstate,
+    pre (spec a pstate) ->
+    forall r, exec p pstate r ->
+         match r with
+         | Finished v pstate' => post (spec a pstate) v pstate'
+         | Crashed pstate' => crash (spec a pstate) pstate'
+         | Failed => False
+         end.
+
+(** Hoare double higher-order precondition *)
+Definition DoublePre T :=
+  (* initial state *)
+  PState ->
+  (* postcondition *)
+  (T -> PState -> Prop) ->
+  (* crash invariant *)
+  (PState -> Prop) ->
+  Prop.
+
+Definition prog_double T (pre: DoublePre T) (p: prog3 T) :=
+  forall pstate postcond crashinv,
+    pre pstate postcond crashinv ->
+    forall r, exec p pstate r ->
+         match r with
+         | Finished v pstate' => postcond v pstate'
+         | Crashed pstate' => crashinv pstate'
+         | Failed => False
+         end.
+
+Definition prog_ok T A (spec: Specification A T) (p: prog3 T) :=
+  forall T' (rx: T -> prog3 T'),
+    prog_double
+      (fun pstate postcond crashinv =>
+         exists a, pre (spec a pstate) /\
+              (forall r, prog_double
+                      (fun pstate' postcond' crashinv' =>
+                         post (spec a pstate) r pstate' /\
+                         postcond' = postcond /\
+                         crashinv' = crashinv)
+                      (rx r)) /\
+              (forall pstate', crash (spec a pstate) pstate' ->
+                          crashinv pstate')) (Bind p rx).
+
+Theorem prog_ok_spec_equiv : forall T A (spec: Specification A T) (p: prog3 T),
+    (forall a pstate r pstate', pre (spec a pstate) ->
+                           post (spec a pstate) r pstate' ->
+                           crash (spec a pstate) pstate') ->
+    prog_ok spec p <-> prog_spec spec p.
+Proof.
+  unfold prog_ok, prog_double, prog_spec; split; intros.
+  - specialize (H0 _ Ret).
+    specialize (H0 pstate).
+    eapply H0.
+    exists a; intuition eauto; subst.
+    match goal with
+    | [ H: exec (Ret _) _ _ |- _ ] =>
+      apply exec_ret in H
+    end.
+    destruct r1; intuition (subst; eauto).
+    apply monad_right_id; auto.
+  - deex.
+    match goal with
+    | [ H: exec (Bind _ _) _ _ |- _ ] =>
+      apply exec_bind in H
+    end.
+    intuition; repeat deex.
+    + eapply H3; intuition eauto.
+      eapply H0 in H2; eauto.
+    + eapply H0 in H2; eauto.
+    + subst.
+      match goal with
+      | [ Hexec: exec _ _ Failed |- _ ] =>
+        eapply H0 in Hexec; eauto
+      end.
+Qed.
+
+Theorem double_weaken : forall T (pre pre': DoublePre T) (p: prog3 T),
+    (forall pstate postcond crashinv, pre pstate postcond crashinv ->
+                                 pre' pstate postcond crashinv) ->
+    prog_double pre' p ->
+    prog_double pre p.
+Proof.
+  unfold prog_double at 2; intros.
+  eapply H0; eauto.
+Qed.
